Risc0/Lemmas.lean
@@ -32,9 +32,33 @@ lemma run_nondet : Γ st ⟦nondet block⟧ = Γ st ⟦block⟧ := rfl
 --   Γ st ⟦⟨"output"⟩[i] ←ᵢ nameₓ⟧ = { st with output := st.output.set i x } := by simp [run_set_def, h₁]
 -- TODO run_set_buffer
 
+lemma run_if' : Γ st ⟦guard ⟨name⟩ then branch⟧
+                = if st.felts ⟨name⟩ = some 0 ∨ ⟨name⟩ ∉ st.felts
+                  then st
+                  else Γ st ⟦branch⟧ := by
+  simp [run]
+  by_cases eq : ⟨name⟩ ∈ st.felts 
+  · have : ∃ a, State.felts st { name := name } = some a := by
+      simp [Map.mem_def, Option.isSome_iff_exists] at eq; exact eq
+    rcases this with ⟨o₁, eq₁⟩; simp [eq₁]
+    by_cases eq₁ : o₁ = 0 <;> simp [eq₁]; simp [eq]
+  · have eq' := eq
+    rw [Map.not_mem_iff_none, Map.getElem_def] at eq
+    simp [eq, eq']
+
 lemma run_if (x : Felt) (h₁ : st.felts ⟨name⟩  = some x) :
   Γ st ⟦guard ⟨name⟩ then branch⟧
   = if x = 0 then st else Γ st ⟦branch⟧ := by simp [run, h₁]
+
+lemma run_eqz' : Γ st ⟦@MLIR.Eqz α ⟨name⟩⟧
+                 = if h : ⟨name⟩ ∈ st.felts
+                   then withEqZero ((st.felts ⟨name⟩).get h) st
+                   else st := by simp [run]
+                                 by_cases eq : ⟨name⟩ ∈ st.felts <;> simp [eq]
+                                 · rw [Map.mem_def, Option.isSome_iff_exists] at eq
+                                   aesop
+                                 · rw [Map.not_mem_iff_none] at eq
+                                   aesop
 
 lemma run_eqz (x : Felt) (h₁ : st.felts ⟨name⟩ = some x) :
   Γ st ⟦@MLIR.Eqz α ⟨name⟩⟧ = withEqZero x st := by simp [run, h₁]
